\documentclass[letterpaper,notitlepage,twoside]{article}

% Basic imports, increase margins...
\usepackage[margin=0.75in]{geometry}
% Finite State Machine stuff

% Format tables nicely
\usepackage[latin1]{inputenc}
\usepackage{array}

\usepackage{amsfonts}
\usepackage{amssymb}
\usepackage{amsmath,amsthm}

\renewcommand{\implies}{\Rightarrow} % redefine command "implies"
\renewcommand{\iff}{\Leftrightarrow} % double arrow
\newcommand{\maps}{\rightarrow} % define command "map"
\newcommand{\union}{\cup}
\newcommand{\intersect}{\cap}
\newcommand{\N}{\mathbb{N}} % natural number
\newcommand{\Q}{\mathbb{Q}} % rational number
\newcommand{\R}{\mathbb{R}} % real number
\newcommand{\Z}{\mathbb{Z}} % integers
\newcommand\tab[1][1cm]{\hspace*{#1}} %\tab command

% Add more packages that you use here...

\begin{document}
\title{Homework 21}
\author{Brian Knotten, Brett Schreiber, Brian Falkenstein}
\maketitle
\section*{6}

\subsection*{3-Sum $\leq_{n \log n}$ 3-Sum-Part}
3-SumAlgorithm($z_1,...z_n$)\\
\tab Let $A = \{z_1,...z_n\}$\\
\tab Let $B = \{z_1,...z_n\}$\\
\tab Let $C = \{z_1,...z_n\}$\\
\tab Return 3-Sum-PartAlgorithm($A, B, C$)
\\\\
Since 3-Sum-Part still contains the restriction that $i \neq j \neq k$, then the existence of a 3-Sum all from one set is equivalent to the existence of a 3-Sum of three equal sets. Since the transformation of the input takes $O(n)$ time, and since there is no transformation of the boolean output, the overall algorithm preserves the $O(n \log n)$ runtime.

\subsection*{3-Sum $\leq_{n \log n}$ 3-Colinear}
This is a reduction we learned in class.
\\\\
3-SumAlgorithm($z_1,...,z_n$):\\
\tab for $i = 1$ to $n$ do:\\
\tab\tab Let $p_i = (z_i, z_i^3)$\\
\tab Return 3-ColinearAlgorithm($p_1,...,p_n$)
\\\\
As discussed in class,
\begin{align*}
a + b + c = 0 &\iff \frac{b^3 - a^3}{b - a} &= \frac{c^3 - b^3}{c - b}\\
&\iff \frac{(b - a)(b^2 + ba + a^2)}{b - a} &= \frac{(c - b)(c^2 + cb + b^2)}{c - b}\\
&\iff b^2 + ba + a^2 &= c^2 + cb + b^2\\
&\iff b^2 + ba + a^2 - c^2 - cb - b^2 &= 0\\
&\iff ba + a^2 - c^2 - cb &= 0\\
&\iff b(a - c) + (a - c)(a + c) &= 0\\
&\iff (a - c)(a + b + c) &= 0\\
&\iff a + b + c &= 0
\end{align*}

\section*{7}
\end{document}
